chkpt
git-svn-id: https://webdav.seas.upenn.edu/svn/sol/vol@3605 eef5ea85-cc2e-0410-bd84-0fae1f012da8

src/Transforms/phiplacement_bsim.v
@@ -34,15 +34,15 @@ forall l0,
   end.
 
 Definition reg_simulation (pinfo: PhiInfo) (f1:fdef) (lc1 lc2:DGVMap) : Prop :=  
-  let '(mkPhiInfo f rd succs preds pid ty al newids) := pinfo in
-  if (fdef_dec f1 f) then 
+  if (fdef_dec (PI_f pinfo) f1) then 
     (forall i0, 
-      not_temporaries i0 newids -> lookupAL _ lc1 i0 = lookupAL _ lc2 i0) 
+      not_temporaries i0 (PI_newids pinfo) -> 
+      lookupAL _ lc1 i0 = lookupAL _ lc2 i0) 
   else lc1 = lc2.
 
 Definition fdef_simulation (pinfo: PhiInfo) f1 f2: Prop :=
   let '(mkPhiInfo f rd succs preds pid ty al _) := pinfo in
-  if (fdef_dec f1 f) then 
+  if (fdef_dec f f1) then 
     phinodes_placement f1 rd pid ty al succs preds = f2
   else f1 = f2.
 
@@ -56,7 +56,7 @@ Definition wf_tmp_value (pinfo: PhiInfo) TD (M2:mem) (lc2:DGVMap) (tid:id)
 Definition cmds_simulation (pinfo: PhiInfo) TD (M2:mem) lc2 (f1:fdef) (b1:block) 
   cs1 cs2 : Prop :=
   let '(mkPhiInfo f rd succs preds pid ty al newids) := pinfo in
-  if (fdef_dec f1 f) then 
+  if (fdef_dec f f1) then 
     let '(block_intro l1 _ cs _) := b1 in 
     match ATree.get l1 newids with
     | Some (lid, pid', sid) =>
@@ -76,11 +76,15 @@ Definition cmds_simulation (pinfo: PhiInfo) TD (M2:mem) lc2 (f1:fdef) (b1:block)
                        exactly after the inserted store in b2;
               moreover, if pid' is inserted, its value should be correct. *)
       (cs = cs1 ->          
-       (cs2 = prefix ++ cs1 ++ suffix \/ cs2 = cs1 ++ suffix) /\ 
-       (prefix <> nil -> wf_tmp_value pinfo TD M2 lc2 pid')) /\
+       (cs2 = prefix ++ cs1 ++ suffix \/ 
+        (prefix <> nil /\ cs2 = cs1 ++ suffix)) /\ 
+       (prefix <> nil -> 
+        cs2 = prefix ++ cs1 ++ suffix ->
+        wf_tmp_value pinfo TD M2 lc2 pid')) /\
       (* If cs1 isn't at the beginning of b1, 
-         then cs2 matches cs1 with suffix. *)
-      (cs <> cs1 -> cs2 = cs1 ++ suffix) /\
+         then cs2 matches cs1 with suffix, or both cs1 and cs2 reach the end *)
+      (cs <> cs1 -> cs2 = cs1 ++ suffix \/ 
+                    (suffix <> nil /\ cs1 = nil /\ cs2 = nil)) /\
       (* Moreover, when both cs1 and cs2 are at the end, and 
                         a load is inserted for b2, 
                    the value of the load shoule be correct. *)
@@ -92,7 +96,7 @@ Definition cmds_simulation (pinfo: PhiInfo) TD (M2:mem) lc2 (f1:fdef) (b1:block)
 
 Definition block_simulation (pinfo: PhiInfo) f1 b1 b2: Prop :=
   let '(mkPhiInfo f _ succs preds pid ty al newids) := pinfo in
-  if (fdef_dec f1 f) then
+  if (fdef_dec f f1) then
      phinodes_placement_block b1 pid ty al newids succs preds = b2
   else b1 = b2.
 
@@ -123,7 +127,7 @@ Definition EC_simulation_head (TD:TargetData) Ps1 (pinfo: PhiInfo)
        InProductsB (product_fdef f1) Ps1 = true /\
        fdef_simulation pinfo f1 f2 /\
        tmn1 = tmn2 /\ als1 = als2 /\
-       (getBlockLabel b1 = getBlockLabel b2) /\
+       block_simulation pinfo f1 b1 b2 /\
        (exists l1, exists ps1, exists cs11, 
          b1 = block_intro l1 ps1 (cs11++cs1) tmn1)
          /\
@@ -143,7 +147,7 @@ Definition EC_simulation_tail (TD:TargetData) Ps1 (pinfo: PhiInfo)
        InProductsB (product_fdef f1) Ps1 = true /\
        fdef_simulation pinfo f1 f2 /\
        tmn1 = tmn2 /\ als1 = als2 /\
-       (getBlockLabel b1 = getBlockLabel b2) /\
+       block_simulation pinfo f1 b1 b2 /\
        (exists l1, exists ps1, exists cs11, 
          b1 = block_intro l1 ps1 (cs11++cs1) tmn1)
          /\
@@ -191,381 +195,29 @@ match (St1, St2) with
     gl1 = gl2 /\ fs1 = fs2 /\ M1 = M2
 end.
 
-(*
-Lemma cmds_simulation_nil_br_inv: forall B F tmn pinfo cs2
-  (HBinF : blockInFdefB B F = true)
-  (Heq: exists l1, exists ps1, exists cs11,
-          B = block_intro l1 ps1 (cs11 ++ nil) tmn)
-  (Hsucc: successors_terminator tmn <> nil)
-  (Htcmds: cmds_simulation pinfo F (getBlockLabel B) nil cs2),
-  if fdef_dec F pinfo.(PI_f) then   
-    match ATree.get (getBlockLabel B) pinfo.(PI_newids) with
-    | None => cs2 = nil
-    | Some (lid', _, _) =>
-        cs2 = [insn_load lid' pinfo.(PI_typ) (value_id pinfo.(PI_id)) 
-                pinfo.(PI_align)]
-    end
-  else
-    cs2 = nil.
-Admitted.
-
-Lemma lookup_fdef_sim__block_sim : forall pinfo f1 f2 l0 b1,
-  fdef_simulation pinfo f1 f2 ->
-  lookupBlockViaLabelFromFdef f1 l0 = Some b1 ->
-  exists b2,
-    lookupBlockViaLabelFromFdef f2 l0 = Some b2 /\
-    block_simulation pinfo f1 b1 b2.
-Admitted.
-
-Lemma simulation__getOperandValue: forall TD v lc gl2 lc2 g F
-  (HeqR : Opsem.getOperandValue TD v lc gl2 = ret g)
-  (Hrsim : reg_simulation F lc lc2),
-  Opsem.getOperandValue TD v lc2 gl2 = ret g.
-Proof.
-  intros.
-  destruct Hrsim as [J1 _].
-  destruct v; auto.
-    apply J1 in HeqR; auto.
-Qed.
-
-Lemma returnUpdateLocals_rsim : forall TD i0 n c t v p Result lc lc' gl2 
-  lc'' F F' lc2' lc2
-  (H1 : Opsem.returnUpdateLocals TD (insn_call i0 n c t v p) Result lc
-         lc' gl2 = ret lc'')
-  (Hrsim : reg_simulation F lc lc2)
-  (Hrsim' : reg_simulation F' lc' lc2'),
-  exists lc2'',
-    Opsem.returnUpdateLocals TD (insn_call i0 n c t v p) Result lc2 lc2' gl2 
-      = ret lc2'' /\ reg_simulation F' lc'' lc2''.
-Proof.
-  unfold Opsem.returnUpdateLocals in *.
-  intros.
-  remember (Opsem.getOperandValue TD Result lc gl2) as R.
-  destruct R; inv H1.
-    destruct n; inv H0.
-    erewrite simulation__getOperandValue; eauto. 
-
-    destruct t; tinv H1.
-    erewrite simulation__getOperandValue; eauto. 
-    destruct (lift_op1 DGVs (fit_gv TD t) g t); inv H1.
-    exists (updateAddAL (GVsT DGVs) lc2' i0 g0).
-    split; auto.
-      destruct Hrsim' as [J1 J2].
-      split; intros.
-        destruct (id_dec i0 i1); subst.
-          rewrite lookupAL_updateAddAL_eq.
-          rewrite lookupAL_updateAddAL_eq in H; auto.
-
-          rewrite <- lookupAL_updateAddAL_neq; auto.
-          rewrite <- lookupAL_updateAddAL_neq in H; auto.
-
-        admit.
-Qed.
-
-(* copied from SB *)
-Lemma cmds_at_block_tail_next : forall B c cs tmn2,
-  (exists l1, exists ps1, exists cs11, B = 
-    block_intro l1 ps1 (cs11 ++ c :: cs) tmn2) ->
-  exists l1, exists ps1, exists cs11, B = block_intro l1 ps1 (cs11 ++ cs) tmn2.
-Proof.
-  intros.
-  destruct H as [l1 [ps1 [cs11 H]]]; subst.
-  exists l1. exists ps1. exists (cs11 ++ [c]). simpl_env. auto.
-Qed.
-
-Ltac destruct_ctx_br :=
-match goal with
-| [Hsim : State_simulation _
-           {|
-           OpsemAux.CurSystem := _;
-           OpsemAux.CurTargetData := ?TD;
-           OpsemAux.CurProducts := _;
-           OpsemAux.Globals := _;
-           OpsemAux.FunTable := _ |}
-           {|
-           Opsem.ECS := {|
-                          Opsem.CurFunction := ?F;
-                          Opsem.CurBB := _;
-                          Opsem.CurCmds := nil;
-                          Opsem.Terminator := _;
-                          Opsem.Locals := _;
-                          Opsem.Allocas := _ |} :: _;
-           Opsem.Mem := _ |} ?Cfg2 ?St2 |- _] =>
-  destruct Cfg2 as [S2 TD2 Ps2 gl2 fs2];
-  destruct St2 as [ECs2 M2];
-  destruct TD as [los nts];
-  destruct Hsim as [Hwfs [HMinS [Htsym [Heq1 [Htps [HsimECs [Heq2 
-    [Heq3 Heq4]]]]]]]]; subst;
-  destruct ECs2 as [|[F2 B2 cs2 tmn2 lc2 als2] ECs2];
-    try solve [inversion HsimECs];
-  simpl in HsimECs;
-  destruct HsimECs as [HsimEC HsimECs];
-  destruct HsimEC as [HBinF [HFinPs [Htfdef [Heq0 [Heq1 [Hnth [Heqb1 [Heqb2     
-    [Hrsim Htcmds]]]]]]]]]; subst
-end.
-
-Lemma phinodes_placement_is_correct__sBranch: forall 
-  (pinfo : PhiInfo) (Cfg2 : OpsemAux.Config) (St2 : Opsem.State)
-  (S : system) (TD : TargetData) (Ps : list product) (F : fdef) (B : block)
-  (lc : Opsem.GVsMap) (gl : GVMap) (fs : GVMap) (bid : id) (Cond : value)
-  (l1 : l) (l2 : l) (ECs : list Opsem.ExecutionContext) (Mem : mem) 
-  (als : list mblock) maxb EC1 Cfg1 (Hwfpi: WF_PhiInfo pinfo)
-  (Heq1: Cfg1 = {| OpsemAux.CurSystem := S;
-                   OpsemAux.CurTargetData := TD;
-                   OpsemAux.CurProducts := Ps;
-                   OpsemAux.Globals := gl;
-                   OpsemAux.FunTable := fs |})
-  (Hnoalias: noalias_EC maxb pinfo TD Mem EC1)
-  (Heq2: EC1 = {| Opsem.CurFunction := F;
-                  Opsem.CurBB := B;
-                  Opsem.CurCmds := nil;
-                  Opsem.Terminator := insn_br bid Cond l1 l2;
-                  Opsem.Locals := lc;
-                  Opsem.Allocas := als |})
-  (Hsim : State_simulation pinfo Cfg1
-            {| Opsem.ECS := EC1 :: ECs;
-               Opsem.Mem := Mem |} Cfg2 St2)
-  (conds : GVsT DGVs) (c : GenericValue) (l' : l) (ps' : phinodes)
-  (cs' : cmds) (tmn' : terminator) (lc' : Opsem.GVsMap)
-  (H : Opsem.getOperandValue TD Cond lc gl = ret conds)
-  (H0 : c @ conds)
-  (H1 : ret block_intro l' ps' cs' tmn' =
-       (if isGVZero TD c
-        then lookupBlockViaLabelFromFdef F l2
-        else lookupBlockViaLabelFromFdef F l1))
-  (H2 : Opsem.switchToNewBasicBlock TD (block_intro l' ps' cs' tmn') B gl lc =
-       ret lc'),
-  exists St2' : Opsem.State,
-     Opsem.sop_plus Cfg2 St2 St2' trace_nil /\
-     State_simulation pinfo Cfg1
-     {|Opsem.ECS := {| Opsem.CurFunction := F;
-                       Opsem.CurBB := (block_intro l' ps' cs' tmn');
-                       Opsem.CurCmds := cs';
-                       Opsem.Terminator := tmn';
-                       Opsem.Locals := lc';
-                       Opsem.Allocas := als |} :: ECs;
-       Opsem.Mem := Mem |} Cfg2 St2'.
-Proof.
-  intros. subst.
-  destruct_ctx_br.
-  assert (exists b2,
-    (if isGVZero (los, nts) c
-     then lookupBlockViaLabelFromFdef F2 l2
-     else lookupBlockViaLabelFromFdef F2 l1) = Some b2 /\
-    block_simulation pinfo F (block_intro l' ps' cs' tmn') b2) as Hfind.
-    symmetry in H1.
-    destruct (isGVZero (los, nts) c); 
-      eapply lookup_fdef_sim__block_sim in H1; eauto.
-  destruct Hfind as [b2 [Hfind Htblock]].
-  eapply cmds_simulation_nil_br_inv in Htcmds; 
-    try solve [eauto | simpl; congruence].
-  destruct (fdef_dec F (PI_f pinfo)) as [ e | n]; subst.
-  SCase "F is tranformed".
-    assert (phinodes_placement_block (block_intro l' ps' cs' tmn') (PI_id pinfo)
-      (PI_typ pinfo) (PI_align pinfo) (PI_newids pinfo) (PI_succs pinfo) 
-      (PI_preds pinfo) = b2) as EQ.
-      clear - Htblock. destruct pinfo. simpl in *.
-      destruct (fdef_dec PI_f0 PI_f0); auto.
-        congruence.
-    subst. clear Htblock. simpl in Hfind.
-    assert ((PI_newids pinfo) ! l' <> None) as Hreach'.
-      admit. (* reachable *)
-    remember ((PI_newids pinfo) ! l') as R1.
-    destruct R1 as [[[lid' pid'] sid']|]; try congruence.
-    assert (exists prd, exists prds, (PI_preds pinfo) ! l' = Some (prd::prds)) 
-      as R2.
-      admit. (* must be of at most one pred *)
-    destruct R2 as [prd [prds Heq]].
-    rewrite Heq in Hfind.
-    assert ((PI_newids pinfo) ! (getBlockLabel B) <> None) as Hreach.
-      admit. (* reachable *)
-    remember ((PI_newids pinfo) ! (getBlockLabel B)) as R.
-    destruct R as [[[lid pid] sid]|]; subst; try congruence.
-    assert (exists mp, exists gv,
-      getOperandValue (los, nts) (value_id (PI_id pinfo)) lc gl2 = Some mp /\
-      mload (los, nts) M2 mp (PI_typ pinfo) (PI_align pinfo) = Some gv) as Halc.
-      clear - Hnoalias.
-      (* By promotablity *)
-      unfold noalias_EC in Hnoalias.
-      destruct (fdef_dec (PI_f pinfo) (PI_f pinfo)); try congruence.
-      assert (exists gvsa, lookupAL _ lc (PI_id pinfo) = Some gvsa) 
-        as Hlkup.
-        (* WF ssa isnt stuck by accessing undefined variables *)
-        admit.
-      destruct Hlkup as [gvsa Hlkup]. simpl. 
-      change (GVsT DGVs) with GenericValue in Hlkup.
-      rewrite Hlkup.
-      apply Hnoalias in Hlkup; auto.
-      destruct Hlkup as [[J1 [J2 [gv J3]]] _].
-      exists gvsa. exists gv. auto.
-    destruct Halc as [mp [gv [Hget Hld]]].
-    assert (reg_simulation (PI_f pinfo) lc 
-             (updateAddAL _ lc2 lid ($ gv # PI_typ pinfo $))) as Hrsim'.
-      admit. (* Hrsim HeqR *)
-    remember (cs' ++ 
-              match (PI_succs pinfo) ! l' with
-              | ret nil => nil
-              | ret (_ :: _) =>
-                  [insn_load lid' (PI_typ pinfo)
-                    (value_id (PI_id pinfo)) (PI_align pinfo)]
-              | merror => nil
-              end) as cs2'.
-    remember (block_intro l'
-                (gen_phinode pid' (PI_typ pinfo) (PI_newids pinfo)
-                   (prd :: prds) :: ps')
-                (insn_store sid' (PI_typ pinfo) (value_id pid')
-                   (value_id (PI_id pinfo)) (PI_align pinfo) :: cs2') tmn') 
-             as b2.
-    assert (exists lc2', 
-      Opsem.switchToNewBasicBlock (los, nts) b2 B2 gl2 
-        (updateAddAL _ lc2 lid ($ gv # PI_typ pinfo $)) = ret lc2' /\
-      reg_simulation (PI_f pinfo) lc' lc2' /\ 
-      lookupAL _ lc2' pid' = Some gv) as Hswitch.
-      admit. (* switch *)
-    destruct Hswitch as [lc2' [Hswitch [Hrsim'' Hlk]]].
-    assert (mstore (los,nts) M2 mp (PI_typ pinfo) gv (PI_align pinfo) 
-      = Some M2) as Hst.
-      clear - Hld. admit. (* By MemModel *)
-    exists (Opsem.mkState ((Opsem.mkEC F2 b2 cs2' tmn' lc2' als2)::ECs2) M2).
-    split.
-    SSCase "opsem".
-      rewrite <- (@trace_app_nil__eq__trace trace_nil).
-      apply Opsem.sop_plus_cons with (state2:=
-         Opsem.mkState 
-           ((Opsem.mkEC F2 B2 nil (insn_br bid Cond l1 l2) 
-             (updateAddAL _ lc2 lid ($ gv # (PI_typ pinfo) $)) als2)::ECs2) M2).
-        eapply simulation__getOperandValue with (lc2:=lc2) in Hget; eauto.
-        econstructor; eauto.
-
-      rewrite <- (@trace_app_nil__eq__trace trace_nil).
-      apply Opsem.sop_star_cons with (state2:=
-         Opsem.mkState 
-           ((Opsem.mkEC F2 b2 
-             (insn_store sid' (PI_typ pinfo) (value_id pid')
-               (value_id (PI_id pinfo)) (PI_align pinfo) :: cs2') 
-             tmn' lc2' als2)::ECs2) M2).
-        subst.
-        eapply simulation__getOperandValue with 
-          (lc2:=updateAddAL _ lc2 lid ($ gv # (PI_typ pinfo) $)) in H; eauto.
-
-      apply OpsemProps.sInsn__implies__sop_star.
-      clear c H0 H1 Hfind.
-      econstructor; eauto.
-        eapply simulation__getOperandValue with (lc:=lc'); eauto.
-          clear - Hget H2.
-          admit. (* By WF promotablity *)
-    SSCase "sim".
-      assert (blockInFdefB (block_intro l' ps' cs' tmn') (PI_f pinfo))as HBinF'.
-        assert (HuniqF:=HFinPs).
-        eapply wf_system__uniqFdef in HuniqF; eauto.
-        destruct (PI_f pinfo) as [[] bs].
-        destruct HuniqF as [HuniqBlocks HuniqArgs].
-        symmetry in H1.
-        destruct (isGVZero (los,nts) c);
-          apply genLabel2Block_blocks_inv with (f:=fheader_intro f t i0 a v) 
-            in H1; auto; destruct H1; eauto.
-      subst.
-      repeat (split; eauto 2 using cmds_at_block_tail_next).
-        exists l'. exists ps'. exists nil. auto.
-
-        exists l'. 
-        exists (gen_phinode pid' (PI_typ pinfo) (PI_newids pinfo) (prd :: prds)
-          :: ps').
-        exists [insn_store sid' (PI_typ pinfo) (value_id pid')
-                 (value_id (PI_id pinfo)) (PI_align pinfo)].
-        simpl_env. auto.
-
-        destruct pinfo. simpl in *.
-        destruct (fdef_dec PI_f0 PI_f0); try congruence.
-          admit. (* WF_PhiInfo *)
-
-  SCase "F isnt tranformed".
-    admit. (* simpl case *)
-Qed.
-*)
-
 Notation "$ gv # t $" := (DGVs.(gv2gvs) gv t) (at level 41).
 
-Definition noalias_EC (maxb:Values.block) (pinfo:PhiInfo) TD M 
-  (ec:Opsem.ExecutionContext) : Prop :=
-let '(Opsem.mkEC f b cs tmn lc als) := ec in
-if (fdef_dec (PI_f pinfo) f) then wf_defs maxb pinfo TD M lc als else True.
-
-Lemma noalias_State__noalias_EC: forall maxb pinfo Cfg EC ECs Mem,
-  Promotability.wf_State maxb pinfo Cfg 
-    {| Opsem.ECS := EC :: ECs; Opsem.Mem := Mem |} ->
-  noalias_EC maxb pinfo (OpsemAux.CurTargetData Cfg) Mem EC.
-Proof.
-  intros. destruct Cfg.
-  destruct H as [[J1 _] _].
-  destruct EC. destruct J1 as [J1 _].
-  simpl. auto.
-Qed.
-
-Ltac destruct_ctx_return :=
-match goal with
-| [Hsim : State_simulation _ ?Cfg1 ?St1 
-           {|
-           OpsemAux.CurSystem := _;
-           OpsemAux.CurTargetData := ?TD;
-           OpsemAux.CurProducts := _;
-           OpsemAux.Globals := _;
-           OpsemAux.FunTable := _ |}
-           {|
-           Opsem.ECS := {|
-                          Opsem.CurFunction := ?F;
-                          Opsem.CurBB := _;
-                          Opsem.CurCmds := nil;
-                          Opsem.Terminator := _;
-                          Opsem.Locals := _;
-                          Opsem.Allocas := _ |}
-                          :: {|
-                             Opsem.CurFunction := ?F';
-                             Opsem.CurBB := _;
-                             Opsem.CurCmds := ?c' :: _;
-                             Opsem.Terminator := _;
-                             Opsem.Locals := _;
-                             Opsem.Allocas := _ |} :: _;
-           Opsem.Mem := _ |} |- _] =>
-  destruct Cfg1 as [S1 TD1 Ps1 gl1 fs1];
-  destruct St1 as [ECs1 M1];
-  destruct TD1 as [los nts];
-  destruct Hsim as [Hwfs [HMinS [Htsym [Heq1 [Htps [HsimECs [Heq2 
-    [Heq3 Heq4]]]]]]]]; subst;
-  destruct ECs1 as [|[F1 B1 cs1 tmn1 lc1 als1] ECs1];
-    try solve [inversion HsimECs];
-  simpl in HsimECs;
-  destruct HsimECs as [HsimEC HsimECs];
-  destruct ECs1 as [|[F1' B1' cs1' tmn1' lc1' als1'] ECs1];
-    try solve [inversion HsimECs];
-  destruct HsimECs as [HsimEC' HsimECs];
-  destruct HsimEC as [HBinF [HFinPs [Htfdef [Heq0 [Heq1 [Hnth [Heqb1 [Heqb2     
-    [Hrsim Htcmds]]]]]]]]]; subst;
-  destruct c'; try solve [inversion HsimEC'];
-  destruct HsimEC' as [HBinF' [HFinPs' [Htfdef' [Heq0' [Heq1' [Hnth' 
-    [Heqb1' [Heqb2' [Hrsim' Htcmds']]]]]]]]]; subst;
-  fold ECs_simulation_tail in HsimECs
-end.
-
-Lemma cmds_simulation_nil_ret_inv: forall TD M2 lc2 F1 B1 cs1 pinfo
+Lemma cmds_simulation_nil_inv: forall TD M2 lc2 F1 B1 cs1 pinfo
   (Htcmds: cmds_simulation pinfo TD M2 lc2 F1 B1 cs1 nil),
   cs1 = nil.
 Proof.
   intros.
-  destruct pinfo. simpl in Htcmds. unfold wf_tmp_value in Htcmds. simpl in Htcmds.
-  destruct (fdef_dec F1 PI_f0); subst; auto.
+  destruct pinfo. simpl in Htcmds. unfold wf_tmp_value in Htcmds. 
+  simpl in Htcmds.
+  destruct (fdef_dec PI_f0 F1); subst; auto.
   destruct B1.
   destruct (PI_newids0 ! l0) as [[[]]|]; auto.
   destruct Htcmds as [J1 [J2 _]].
   destruct (list_eq_dec cmd_dec c cs1).
     apply J1 in e. 
-    destruct e as [[e | e] _];
+    destruct e as [[e | [_ e]] _];
       repeat match goal with
       | H : nil = _ ++ _ |- _ => symmetry in H
       | H : _ ++ _ = nil |- _ => apply app_eq_nil in H; destruct H; auto
       end.
 
     apply J2 in n.
+    destruct n as [n | [_ [n _]]]; auto.
     repeat match goal with
     | H : nil = _ ++ _ |- _ => symmetry in H
     | H : _ ++ _ = nil |- _ => apply app_eq_nil in H; destruct H; auto
@@ -594,7 +246,7 @@ match c with
 | _ => True
 end.
 
-Ltac cmds_simulation_cons_inv_tac2 :=
+Ltac cmds_simulation_same_cons_inv_tac2 :=
 let foo e cs1 Hnoldst l0 HeqR :=
     simpl_env in e;
     destruct cs1; inv e; 
@@ -618,16 +270,17 @@ match goal with
   match goal with
   | e : ?c :: ?cs2 = nil ++ ?cs1 ++ [insn_load _ _ _ _] |- _ => 
       foo e cs1 Hnoldst l0 HeqR
-  | e : ?c :: ?cs2 = ?cs1 ++ [insn_load _ _ _ _] |- _ => foo e cs1 Hnoldst l0 HeqR
+  | e : ?c :: ?cs2 = ?cs1 ++ [insn_load _ _ _ _] |- _ => 
+      foo e cs1 Hnoldst l0 HeqR
   end
 end.
 
-Ltac cmds_simulation_cons_inv_tac3 R2 :=
+Ltac cmds_simulation_same_cons_inv_tac3 R2 :=
  let l2 := fresh "l2" in
  destruct R2 as [l2|]; try solve [
    destruct l2; try solve 
      [cmds_simulation_cons_inv_tac1|
-      cmds_simulation_cons_inv_tac2] |
+      cmds_simulation_same_cons_inv_tac2] |
    cmds_simulation_cons_inv_tac1].
 
 Lemma app_cons_is_larger: forall A cs3 cs2 (c:A),
@@ -648,9 +301,86 @@ Lemma cmds_simulation_other_cons_inv: forall pinfo TD M2 lc2 F1 B1 cs1 c cs2
 Proof.
   intros.
   destruct pinfo. simpl in *. unfold wf_tmp_value in *. simpl in *.
-  destruct (fdef_dec F1 PI_f0); subst; try congruence.
+  destruct (fdef_dec PI_f0 F1); subst; try congruence.
   eauto.
 Qed.
+
+Lemma app_inv_tail_nil : forall A (l1 l2:list A),
+  l1 ++ l2 = l2 -> l1 = nil.
+Proof.
+  intros.
+  change l2 with (nil ++ l2) in H at 2.
+  apply app_inv_tail in H; auto.
+Qed.
+
+
+Ltac cmds_simulation_cons_inv_tac1' :=
+let foo cs2 e :=
+    exists cs2;
+    rewrite e; simpl_env;
+    split; try solve [
+      auto |
+      split; intros; subst; try solve [
+        split; try solve [
+          auto |
+          intros;
+          match goal with
+          | H0: ?cs2 = [_] ++ ?cs2 |- _ =>
+            symmetry in H0; apply app_inv_tail_nil in H0; congruence
+          end] | 
+        split; try solve [auto | intros; congruence]
+      ]
+    ] in
+match goal with
+| e : ?c :: ?cs2 = ?cs1 ++ nil |- _ => foo cs2 e
+| e : ?c :: ?cs2 = nil ++ ?cs1 ++ nil |- _ => foo cs2 e
+end.
+
+Ltac cmds_simulation_same_cons_inv_tac2' :=
+let foo e cs1 Hnoldst l0 HeqR :=
+    simpl_env in e;
+    destruct cs1; inv e; 
+      try solve [
+        assert (J:=Hnoldst l0); simpl in J; rewrite <- HeqR in J;
+        destruct J as [J7 [J8 J9]]; try congruence];
+    exists cs1;
+    split; try solve [
+      auto |
+      split; intros; subst; try solve [
+        split; try solve [
+          auto |
+          intros;
+          match goal with
+          | H0: ?cs2 = [_] ++ ?cs2 |- _ =>
+            symmetry in H0; apply app_inv_tail_nil in H0; congruence
+          end] |
+        split; try solve [
+          auto | 
+          intros; subst;
+          match goal with
+          | H1 : nil ++ [_] = nil |- _ => inv H1
+          end
+        ]
+      ]
+    ] in
+match goal with
+| Hnoldst : isnt_inserted_ldst _ ?c,
+  HeqR : Some (_, _, _) = _ ! ?l0 |- _ => 
+  match goal with
+  | e : ?c :: ?cs2 = nil ++ ?cs1 ++ [insn_load _ _ _ _] |- _ => 
+      foo e cs1 Hnoldst l0 HeqR
+  | e : ?c :: ?cs2 = ?cs1 ++ [insn_load _ _ _ _] |- _ => 
+      foo e cs1 Hnoldst l0 HeqR
+  end
+end.
+
+Ltac cmds_simulation_same_cons_inv_tac3' R2 :=
+ let l2 := fresh "l2" in
+ destruct R2 as [l2|]; try solve [
+   destruct l2; try solve 
+     [cmds_simulation_cons_inv_tac1'|
+      cmds_simulation_same_cons_inv_tac2'] |
+   cmds_simulation_cons_inv_tac1'].
 
 Lemma cmds_simulation_same_cons_inv: forall pinfo TD M2 lc2 F1 B1 cs1 c cs2
   (Htcmds: cmds_simulation pinfo TD M2 lc2 F1 B1 cs1 (c::cs2))
@@ -664,7 +394,7 @@ Lemma cmds_simulation_same_cons_inv: forall pinfo TD M2 lc2 F1 B1 cs1 c cs2
 Proof.
   intros.
   destruct pinfo. simpl in *. unfold wf_tmp_value in *. simpl in *.
-  destruct (fdef_dec F1 PI_f0); subst; try congruence.
+  destruct (fdef_dec PI_f0 F1); subst F1; try congruence.
   destruct B1.
   remember (PI_newids0 ! l0) as R.
   destruct R as [[[]]|]; eauto.
@@ -674,17 +404,20 @@ Proof.
   destruct (list_eq_dec cmd_dec c0 cs1).
   Case "1".
     clear J2. apply_clear J1 in e. 
-    destruct e as [[e | e] J4];
+    destruct e as [[e | [ e1 e]] J4];
       destruct R1 as [l1|]; try solve [
         destruct l1; try solve [
-          cmds_simulation_cons_inv_tac3 R2 | 
+          cmds_simulation_same_cons_inv_tac3 R2 | 
+          cmds_simulation_same_cons_inv_tac3' R2 | 
           inv e; assert (J:=Hnoldst l0); simpl in J; rewrite <- HeqR in J;
             destruct J as [J7 [J8 J9]]; try congruence ] | 
-        cmds_simulation_cons_inv_tac3 R2].
+        cmds_simulation_same_cons_inv_tac3 R2 |
+        cmds_simulation_same_cons_inv_tac3' R2].
 
   Case "2".
     assert (n':=n).
     apply J2 in n. 
+    destruct n as [n | [_ [_ n]]]; try congruence.
     destruct R2 as [l2|].
     SCase "2.1".    
       destruct l2.
@@ -696,6 +429,7 @@ Proof.
          SSSCase "2.1.1.1".    
           destruct l1.
           SSSSCase "2.1.1.1.1".    
+            simpl_env.
             split; intros;
               split; try solve [auto | intros; congruence].
             split; intros.
@@ -754,6 +488,7 @@ Proof.
         SSCase "2.2.1".    
           destruct l1.
           SSSCase "2.2.1.1".    
+            simpl_env.
             split; intros;
               split; try solve [auto | intros; congruence].
           SSSCase "2.2.1.2".    
@@ -826,30 +561,65 @@ Proof.
   exists l0. exists ps0. exists tmn0. exists i1. exists i2. exists i3.
   remember (PI_preds0 ! l0) as R1.
   remember (PI_succs0 ! l0) as R2.
+
+Ltac cmds_simulation_same_head_inv_tac :=
+match goal with 
+| Hin : blockInFdefB _ _ = true,
+  J1 : insn_store ?i0 ?t ?v ?v0 ?a :: _ = 
+       ?cs1 ++ 
+       match ?R2 with
+       | ret _ => _
+       | merror => _
+       end |- _ => 
+  assert (exists cs1', cs1 = insn_store i0 t v v0 a :: cs1') as EQ;
+    destruct cs1; try solve [
+      destruct R2 as [[]|]; inv J1 |
+      inv J1; eauto];
+  destruct EQ as [cs1' EQ]; inv EQ; subst;
+  eapply temporary_must_be_fresh in Hin; eauto; inv Hin
+end.
+
   destruct (list_eq_dec cmd_dec (cs0++cs1) cs1).
   Case "1".
-    assert (cs0 = nil) as EQ. admit. clear e0.
-    subst cs0.
+    apply app_inv_tail_nil in e0; subst cs0.
     split; auto.
     split; auto.
     clear J2.
     destruct J1 as [J1 _]; auto.
-    destruct J1 as [J1 | J1].
-      destruct R1.
-        destruct l1.  
-          admit.
+    destruct J1 as [J1 | [_ J1]].
+      destruct R1; simpl in J1.
+        destruct l1; simpl in J1.
+          cmds_simulation_same_head_inv_tac.
 
-          inv J1. 
+          inv J1.
           split; auto.
           split; intros; congruence.
-        admit.
-      admit.
+
+        cmds_simulation_same_head_inv_tac.
+      cmds_simulation_same_head_inv_tac.
 
   Case "2".
     clear J1.
     apply_clear J2 in n.
-    admit.
+    destruct n as [n | [_ [_ n]]]; try congruence.
+    cmds_simulation_same_head_inv_tac.
 Qed.
+
+Ltac cmds_simulation_tail_inv_tac :=
+match goal with 
+| Hin : blockInFdefB _ _ = true,
+  J1 : insn_load ?i0 ?t ?v ?a :: _ = 
+       ?cs1 ++ 
+       match ?R2 with
+       | ret _ => _
+       | merror => _
+       end |- _ => 
+    destruct cs1; try solve [
+      inv J1; eapply temporary_must_be_fresh in Hin; eauto; inv Hin |
+      destruct R2 as [[]|]; inv J1;
+        repeat split; try solve [auto | intros; congruence]
+      ]
+end.
 
 Lemma cmds_simulation_tail_inv: forall pinfo TD M2 lc2 F1 B1 cs1 c cs2
   (Hin: blockInFdefB B1 F1 = true) (Hwfpi: WF_PhiInfo pinfo)
@@ -880,28 +650,786 @@ Proof.
   remember (PI_succs0 ! l0) as R2.
   destruct (list_eq_dec cmd_dec (cs0++cs1) cs1).
   Case "1".
-    assert (cs0 = nil) as EQ. admit. clear e0.
-    subst cs0.
-    clear J2.
+    apply app_inv_tail_nil in e0; subst cs0.
     destruct J1 as [J1 _]; auto.
-    destruct J1 as [J1 | J1].
-      destruct R1.
-        destruct l1.  
+    destruct J1 as [J1 | [_ J1]].
+      destruct R1; simpl in J1.
+        destruct l1; tinv J1.
           destruct cs1.
             destruct R2; tinv J1.
               destruct l1; inv J1.
               repeat split; try solve [auto | intros; congruence]. 
-            admit.
-
-          inv J1. 
-        admit.
-      admit.
+            inv J1.
+            eapply temporary_must_be_fresh in Hin; eauto; inv Hin.
+        cmds_simulation_tail_inv_tac.
+      cmds_simulation_tail_inv_tac.
 
   Case "2".
     clear J1.
     apply_clear J2 in n.
-    admit.
+    destruct n as [n | [_ [_ n]]]; try congruence.
+    cmds_simulation_tail_inv_tac.
 Qed.
+
+Definition isnt_ldst c : Prop :=
+match c with
+| insn_load _ _ _ _ | insn_store _ _ _ _ _ => False
+| _ => True
+end.
+
+Ltac cmds_simulation_non_ldst_cons_inv_tac2 :=
+let foo e cs1 Hnoldst l0 HeqR :=
+    simpl_env in e;
+    destruct cs1; inv e; tinv Hnoldst;
+    exists cs1;
+    split; try solve 
+      [auto |
+       split; intros; 
+       split; auto; try solve [
+         intros; subst;
+         match goal with
+         | H1 : nil ++ [_] = nil |- _ => inv H1
+         end
+         ]
+      ] in
+match goal with
+| Hnoldst : isnt_ldst ?c,
+  HeqR : Some (_, _, _) = _ ! ?l0 |- _ => 
+  match goal with
+  | e : ?c :: ?cs2 = nil ++ ?cs1 ++ [insn_load _ _ _ _] |- _ => 
+      foo e cs1 Hnoldst l0 HeqR
+  | e : ?c :: ?cs2 = ?cs1 ++ [insn_load _ _ _ _] |- _ => 
+      foo e cs1 Hnoldst l0 HeqR
+  end
+end.
+
+Ltac cmds_simulation_non_ldst_cons_inv_tac2' :=
+let foo e cs1 Hnoldst l0 HeqR :=
+    simpl_env in e;
+    destruct cs1; inv e; tinv Hnoldst;
+    exists cs1;
+    split; try solve [
+      auto |
+      split; intros; subst; try solve [
+        split; try solve [
+          auto |
+          intros;
+          match goal with
+          | H0: ?cs2 = [_] ++ ?cs2 |- _ =>
+            symmetry in H0; apply app_inv_tail_nil in H0; congruence
+          end] |
+        split; try solve [
+          auto | 
+          intros; subst;
+          match goal with
+          | H1 : nil ++ [_] = nil |- _ => inv H1
+          end
+        ]
+      ]
+    ] in
+match goal with
+| Hnoldst : isnt_ldst ?c,
+  HeqR : Some (_, _, _) = _ ! ?l0 |- _ => 
+  match goal with
+  | e : ?c :: ?cs2 = nil ++ ?cs1 ++ [insn_load _ _ _ _] |- _ => 
+      foo e cs1 Hnoldst l0 HeqR
+  | e : ?c :: ?cs2 = ?cs1 ++ [insn_load _ _ _ _] |- _ => 
+      foo e cs1 Hnoldst l0 HeqR
+  end
+end.
+
+Ltac cmds_simulation_non_ldst_cons_inv_tac3 R2 :=
+ let l2 := fresh "l2" in
+ destruct R2 as [l2|]; try solve [
+   destruct l2; try solve 
+     [cmds_simulation_cons_inv_tac1|
+      cmds_simulation_non_ldst_cons_inv_tac2] |
+   cmds_simulation_cons_inv_tac1].
+
+Ltac cmds_simulation_non_ldst_cons_inv_tac3' R2 :=
+ let l2 := fresh "l2" in
+ destruct R2 as [l2|]; try solve [
+   destruct l2; try solve 
+     [cmds_simulation_cons_inv_tac1'|
+      cmds_simulation_non_ldst_cons_inv_tac2'] |
+   cmds_simulation_cons_inv_tac1'].
+
+Lemma cmds_simulation_non_ldst_cons_inv: forall pinfo TD M2 lc2 F1 B1 cs1 c cs2
+  (Htcmds: cmds_simulation pinfo TD M2 lc2 F1 B1 cs1 (c::cs2))
+  (Heq: exists l0, exists ps0, exists cs0, exists tmn0, 
+          B1 = block_intro l0 ps0 (cs0++cs1) tmn0)
+  (Hnoldst: isnt_ldst c),
+  exists cs1', 
+    cs1 = c::cs1' /\   
+    cmds_simulation pinfo TD M2 lc2 F1 B1 cs1' cs2.
+Proof.
+  intros.
+  destruct pinfo. simpl in *. unfold wf_tmp_value in *. simpl in *.
+  destruct (fdef_dec PI_f0 F1); subst; eauto.
+  destruct B1.
+  remember (PI_newids0 ! l0) as R.
+  destruct R as [[[]]|]; eauto.
+  destruct Htcmds as [J1 [J2 J3]].
+  remember (PI_preds0 ! l0) as R1.
+  remember (PI_succs0 ! l0) as R2.
+  destruct (list_eq_dec cmd_dec c0 cs1).
+  Case "1".
+    clear J2. apply_clear J1 in e. 
+    destruct e as [[e | [e1 e]] J4];
+      destruct R1 as [l1|]; try solve [
+        destruct l1; try solve [
+          cmds_simulation_non_ldst_cons_inv_tac3 R2 | 
+          cmds_simulation_non_ldst_cons_inv_tac3' R2 | 
+          inv e; inv Hnoldst ] | 
+        cmds_simulation_non_ldst_cons_inv_tac3 R2 |
+        cmds_simulation_non_ldst_cons_inv_tac3' R2].
+  
+  Case "2".
+    assert (n':=n).
+    apply J2 in n. 
+    destruct n as [n | [_ [_ n]]]; try congruence.
+    destruct R2 as [l2|].
+    SCase "2.1".    
+      destruct l2.
+      SSCase "2.1.1".    
+        exists cs2.
+        simpl_env in n. subst cs1.
+        split; auto.
+        destruct R1 as [l1|].
+         SSSCase "2.1.1.1".    
+          destruct l1.
+          SSSSCase "2.1.1.1.1".    
+            simpl_env.
+            split; intros;
+              split; try solve [auto | intros; congruence].
+            split; intros.
+              subst. destruct Heq as [l3 [ps3 [cs3 [tmn3 Heq]]]].
+              inversion Heq.
+              apply app_cons_is_larger in H2. inv H2.
+
+          SSSSCase "2.1.1.1.2".    
+             split; try solve [auto | intros; congruence].
+        SSSCase "2.1.1.2".    
+        split; intros.
+          subst. destruct Heq as [l3 [ps3 [cs3 [tmn3 Heq]]]].
+          inversion Heq.
+          apply app_cons_is_larger in H2. inv H2.
+
+          split; try solve [auto | intros; congruence].
+          
+      SSCase "2.1.2".    
+        destruct cs1; inversion n.
+        SSSCase "2.1.2.1".    
+          subst c. inv Hnoldst.
+
+        SSSCase "2.1.2.2".    
+          exists cs1.
+          split; auto.
+          destruct R1 as [l3|].
+          SSSSCase "2.1.2.2.1".    
+            destruct l3.
+            SSSSSCase "2.1.2.2.1.1".    
+              split; intros;
+                split; try solve [auto | intros; congruence].
+              intros. subst. inv H3.
+
+            SSSSSCase "2.1.2.2.1.2".    
+              split; intros.
+                subst. destruct Heq as [l5 [ps3 [cs3 [tmn3 Heq]]]].
+                inversion Heq.
+                apply app_cons_is_larger in H2. inv H2.
+              split; auto.
+                intros. subst. inv H3.
+
+          SSSSCase "2.1.2.2.2".    
+            split; intros; auto.
+            split; intros; auto.
+              congruence.
+            split; intros; auto.
+              subst. inv H3.
+
+    SCase "2.2".    
+        exists cs2.
+        simpl_env in n. subst cs1.
+        split; auto.
+        destruct R1 as [l1|].
+        SSCase "2.2.1".    
+          destruct l1.
+          SSSCase "2.2.1.1".    
+            simpl_env.
+            split; intros;
+              split; try solve [auto | intros; congruence].
+          SSSCase "2.2.1.2".    
+            split; intros.
+              subst. destruct Heq as [l3 [ps3 [cs3 [tmn3 Heq]]]].
+              inversion Heq.
+              apply app_cons_is_larger in H2. inv H2.
+
+              split; try solve [auto | intros; congruence].
+        SSCase "2.2.2".    
+          split; intros.
+            subst. destruct Heq as [l3 [ps3 [cs3 [tmn3 Heq]]]].
+            inversion Heq.
+            apply app_cons_is_larger in H2. inv H2.
+
+            split; try solve [auto | intros; congruence].
+Qed.
+
+Definition value_has_no_tmps (pinfo:PhiInfo) (v:value) : Prop :=
+match v with
+| value_const _ => True
+| value_id vid => not_temporaries vid (PI_newids pinfo)
+end.
+
+Lemma simulation__getOperandValue: forall pinfo TD v lc gl2 lc2 F
+  (Hntmp: if fdef_dec (PI_f pinfo) F then value_has_no_tmps pinfo v else True)
+  (Hrsim : reg_simulation pinfo F lc lc2),
+  Opsem.getOperandValue TD v lc gl2 = Opsem.getOperandValue TD v lc2 gl2.
+Proof.
+  intros.
+  destruct v; auto.
+    unfold reg_simulation in Hrsim.
+    destruct (fdef_dec (PI_f pinfo) F); subst; auto.
+    simpl in *. eauto.
+Qed.
+
+Lemma returnUpdateLocals_rsim : forall pinfo TD i0 n c t v p Result lc2 lc2' gl2 
+  lc2'' F F' lc1' lc1
+  (Hntmp: if fdef_dec (PI_f pinfo) F then value_has_no_tmps pinfo Result 
+          else True)
+  (H1 : Opsem.returnUpdateLocals TD (insn_call i0 n c t v p) Result lc2
+         lc2' gl2 = ret lc2'')
+  (Hrsim : reg_simulation pinfo F lc1 lc2)
+  (Hrsim' : reg_simulation pinfo F' lc1' lc2'),
+  exists lc1'',
+    Opsem.returnUpdateLocals TD (insn_call i0 n c t v p) Result lc1 lc1' gl2 
+      = ret lc1'' /\ reg_simulation pinfo F' lc1'' lc2''.
+Proof.
+  unfold Opsem.returnUpdateLocals in *.
+  intros.
+  inv_mbind'.
+  erewrite simulation__getOperandValue; eauto. 
+  rewrite <- HeqR. 
+  destruct n; inv H0; eauto.
+    destruct t; tinv H1.
+    inv_mbind'.
+    exists (updateAddAL (GVsT DGVs) lc1' i0 g0).
+    split; auto.
+      unfold reg_simulation in *.
+      destruct (fdef_dec (PI_f pinfo) F'); subst; auto.
+        intros.
+        apply Hrsim' in H.
+        destruct (id_dec i0 i1); subst.
+          repeat rewrite lookupAL_updateAddAL_eq. auto.
+          repeat rewrite <- lookupAL_updateAddAL_neq; auto.
+Qed.
+
+Lemma original_values_arent_tmps: forall pinfo F B v instr
+  (Hwfpi: WF_PhiInfo pinfo) 
+  (HBinF : insnInFdefBlockB instr F B = true)
+  (HvInOps : valueInInsnOperands v instr),
+  if fdef_dec (PI_f pinfo) F then value_has_no_tmps pinfo v else True.
+Proof.
+  intros.
+  destruct (fdef_dec (PI_f pinfo) F); subst; auto.
+  destruct v; simpl; auto.
+  destruct pinfo; simpl in *.  
+  destruct Hwfpi as [_ [_ [_ [_ Hfresh]]]].
+  intros l0.
+  rewrite Hfresh.
+  remember ((fst (gen_fresh_ids PI_rd0 (getFdefLocs PI_f0))) ! l0) as R.
+  destruct R as [[[]]|]; auto.
+Admitted.
+
+Ltac solve_tmnInFdefBlockB :=
+match goal with
+| Heqb1 : exists _, exists _, exists _,
+            ?B1 = block_intro _ _ _ ?tmn,
+  HBinF : blockInFdefB ?B1 ?F1 = true |- 
+  terminatorInBlockB ?tmn ?B1 && blockInFdefB ?B1 ?F1 = true =>
+    destruct Heqb1 as [l1 [ps1 [cs11 Heqb1]]]; subst;
+    simpl;
+    apply andb_true_iff;
+    split; try solve [auto | apply terminatorEqB_refl]
+end.
+
+(* copied from SB *)
+Lemma cmds_at_block_tail_next : forall B c cs tmn2,
+  (exists l1, exists ps1, exists cs11, B = 
+    block_intro l1 ps1 (cs11 ++ c :: cs) tmn2) ->
+  exists l1, exists ps1, exists cs11, B = block_intro l1 ps1 (cs11 ++ cs) tmn2.
+Proof.
+  intros.
+  destruct H as [l1 [ps1 [cs11 H]]]; subst.
+  exists l1. exists ps1. exists (cs11 ++ [c]). simpl_env. auto.
+Qed.
+
+Ltac destruct_ctx_return :=
+match goal with
+| [Hsim : State_simulation _ ?Cfg1 ?St1 
+           {|
+           OpsemAux.CurSystem := _;
+           OpsemAux.CurTargetData := ?TD;
+           OpsemAux.CurProducts := _;
+           OpsemAux.Globals := _;
+           OpsemAux.FunTable := _ |}
+           {|
+           Opsem.ECS := {|
+                          Opsem.CurFunction := ?F;
+                          Opsem.CurBB := _;
+                          Opsem.CurCmds := nil;
+                          Opsem.Terminator := _;
+                          Opsem.Locals := _;
+                          Opsem.Allocas := _ |}
+                          :: {|
+                             Opsem.CurFunction := ?F';
+                             Opsem.CurBB := _;
+                             Opsem.CurCmds := ?c' :: _;
+                             Opsem.Terminator := _;
+                             Opsem.Locals := _;
+                             Opsem.Allocas := _ |} :: _;
+           Opsem.Mem := _ |} |- _] =>
+  destruct Cfg1 as [S1 TD1 Ps1 gl1 fs1];
+  destruct St1 as [ECs1 M1];
+  destruct TD1 as [los nts];
+  destruct Hsim as [Hwfs [HMinS [Htsym [Heq1 [Htps [HsimECs [Heq2 
+    [Heq3 Heq4]]]]]]]]; subst;
+  destruct ECs1 as [|[F1 B1 cs1 tmn1 lc1 als1] ECs1];
+    try solve [inversion HsimECs];
+  simpl in HsimECs;
+  destruct HsimECs as [HsimEC HsimECs];
+  destruct ECs1 as [|[F1' B1' cs1' tmn1' lc1' als1'] ECs1];
+    try solve [inversion HsimECs];
+  destruct HsimECs as [HsimEC' HsimECs];
+  destruct HsimEC as [HBinF [HFinPs [Htfdef [Heq0 [Heq1 [Hbsim [Heqb1 [Heqb2     
+    [Hrsim Htcmds]]]]]]]]]; subst;
+  destruct c'; try solve [inversion HsimEC'];
+  destruct HsimEC' as [HBinF' [HFinPs' [Htfdef' [Heq0' [Heq1' [Hbsim' 
+    [Heqb1' [Heqb2' [Hrsim' Htcmds']]]]]]]]]; subst;
+  fold ECs_simulation_tail in HsimECs
+end.
+
+Lemma cmds_simulation_stable: forall pinfo TD Mem lc' F1' l1 ps1 cs11 c cs1'0 
+  tmn' cs' lc'' Mem' l2 ps2 cs21 (Hwfpi: WF_PhiInfo pinfo)
+  (Hin : blockInFdefB (block_intro l1 ps1 (cs11 ++ c :: cs1'0) tmn') F1' = true)
+  (Hbsim: block_simulation pinfo F1' 
+    (block_intro l1 ps1 (cs11 ++ c :: cs1'0) tmn') 
+    (block_intro l2 ps2 (cs21 ++ c :: cs') tmn')),
+  cmds_simulation pinfo TD Mem lc' F1' 
+    (block_intro l1 ps1 (cs11 ++ c :: cs1'0) tmn') 
+    cs1'0 cs' ->
+  cmds_simulation pinfo TD Mem' lc'' F1' 
+    (block_intro l1 ps1 (cs11 ++ c :: cs1'0) tmn') 
+    cs1'0 cs'.
+Proof.
+  destruct pinfo.
+  simpl. intros.
+  destruct (fdef_dec PI_f0 F1'); subst; auto.
+  remember (PI_newids0 ! l1) as R.
+  destruct R as [[[]]|]; auto.
+  destruct H as [J1 [J2 J3]].
+  split; intros.
+    symmetry in H.
+    apply app_cons_is_larger in H. inv H.
+  split; auto.
+    intros; subst.
+    destruct (PI_succs0 ! l1) as [succs|]; try congruence.
+    destruct succs; try congruence.
+    destruct Hwfpi as [Hwfpi1 [Hwfpi2 [Hwfpi3 [Hwfpi4 Hwfpi5]]]]; subst.
+    assert (Hit: is_temporary
+      (getCmdLoc (insn_load i0 PI_typ0 (value_id PI_id0) PI_align0))
+      (fst (gen_fresh_ids PI_rd0 (getFdefLocs F1')))).
+      simpl.
+      exists l1. rewrite <- HeqR.
+      left.
+      destruct (i0 == i0); simpl; auto; try congruence.
+
+Ltac cmds_simulation_stable_tac :=
+match goal with
+| H3 : _ ++ [_] = _ ++ _ :: nil,
+  Hin : blockInFdefB _ _ = true |- _ =>
+      apply app_inj_tail in H3;
+      destruct H3; subst;
+      eapply temporary_must_be_fresh in Hin; eauto; inv Hin
+end.
+
+    destruct (@ATree.get (list l) l1 (make_predecessors (successors F1')))
+      as [[]|]; inv Hbsim; try cmds_simulation_stable_tac.
+
+      rewrite_env 
+        ((insn_store i2 PI_typ0 (value_id i1) (value_id PI_id0) PI_align0 ::
+         cs11 ++ c :: nil) ++
+        [insn_load i0 PI_typ0 (value_id PI_id0) PI_align0]) in H3.
+      cmds_simulation_stable_tac.
+Qed.     
+
+Lemma cmds_simulation_tail_stable: forall pinfo TD Mem lc' F1' l1 ps1 cs11 c 
+  cs12 tmn' cs' lc'' Mem' l2 ps2 cs21 (Hwfpi: WF_PhiInfo pinfo)
+  (Hnt : isnt_ldst c)
+  (Hin : blockInFdefB (block_intro l1 ps1 (cs11 ++ cs12) tmn') F1' = true)
+  (Hbsim: block_simulation pinfo F1' 
+    (block_intro l1 ps1 (cs11 ++ cs12) tmn') 
+    (block_intro l2 ps2 (cs21 ++ c :: cs') tmn')),
+  cmds_simulation pinfo TD Mem lc' F1' 
+    (block_intro l1 ps1 (cs11 ++ cs12) tmn') 
+    cs12 (c::cs') ->
+  cmds_simulation pinfo TD Mem' lc'' F1' 
+    (block_intro l1 ps1 (cs11 ++ cs12) tmn') 
+    cs12 (c::cs').
+Proof.
+  destruct pinfo.
+  simpl. intros.
+  destruct (fdef_dec PI_f0 F1'); subst; auto.
+  remember (PI_newids0 ! l1) as R.
+  destruct R as [[[]]|]; auto.
+  destruct H as [J1 [J2 J3]].
+  split; intros.
+    assert (W:=H).
+    apply app_inv_tail_nil in H. subst cs11.
+    apply J1 in W. clear J1.
+    destruct W as [W1 W2].
+    split; auto.
+      intros W3 W4.
+      destruct (PI_preds0 ! l1) as [[]|]; try congruence.
+      clear J2 J3.
+      destruct W1 as [W1 | [ W1' W1]].
+        inv W1. inv Hnt.
+
+        rewrite W1 in Hbsim.
+        simpl_env in Hbsim.
+        inv Hbsim.
+        simpl_env in H2.
+        apply app_inv_tail in H2; subst.    
+        inv W4. inv Hnt.
+
+  split; auto.
+    intros; subst.
+    destruct (PI_succs0 ! l1) as [succs|]; try congruence.
+Qed.     
+
+Lemma EC_simulation_tail_stable: forall TD Ps1 pinfo Mem Mem' EC1 EC2
+  (Hwfpi: WF_PhiInfo pinfo)
+  (H: EC_simulation_tail TD Ps1 pinfo EC1 EC2 Mem),
+  EC_simulation_tail TD Ps1 pinfo EC1 EC2 Mem'.
+Proof.
+  destruct EC1. destruct EC2. destruct TD. intros.
+  destruct CurCmds0 as [|[]]; simpl; auto.
+  destruct H as [J1 [J2 [J3 [J4 [J5 [J6 [J7 [J8 [J9 J10]]]]]]]]].
+  repeat split; auto.
+    destruct J7 as [l1 [ps1 [cs11 J7]]]; subst.
+    destruct J8 as [l2 [ps2 [cs21 J8]]]; subst.
+    eapply cmds_simulation_tail_stable; simpl; eauto.
+Qed.
+
+Lemma ECs_simulation_tail_stable: forall TD Ps1 pinfo Mem Mem' ECs1 ECs2
+  (Hwfpi: WF_PhiInfo pinfo),
+  ECs_simulation_tail TD Ps1 pinfo ECs1 ECs2 Mem ->
+  ECs_simulation_tail TD Ps1 pinfo ECs1 ECs2 Mem'.
+Proof.
+  induction ECs1; destruct ECs2; simpl; intros; auto.
+    destruct H.
+    split; eauto.
+      eapply EC_simulation_tail_stable; eauto.
+Qed.
+
+Definition noalias_EC (maxb:Values.block) (pinfo:PhiInfo) TD M 
+  (ec:Opsem.ExecutionContext) : Prop :=
+let '(Opsem.mkEC f b cs tmn lc als) := ec in
+if (fdef_dec (PI_f pinfo) f) then wf_defs maxb pinfo TD M lc als else True.
+
+Lemma noalias_State__noalias_EC: forall maxb pinfo Cfg EC ECs Mem,
+  Promotability.wf_State maxb pinfo Cfg 
+    {| Opsem.ECS := EC :: ECs; Opsem.Mem := Mem |} ->
+  noalias_EC maxb pinfo (OpsemAux.CurTargetData Cfg) Mem EC.
+Proof.
+  intros. destruct Cfg.
+  destruct H as [[J1 _] _].
+  destruct EC. destruct J1 as [J1 _].
+  simpl. auto.
+Qed.
+
+Ltac destruct_ctx_br :=
+match goal with
+| [Hsim : State_simulation _ ?Cfg1 ?St1
+           {|
+           OpsemAux.CurSystem := _;
+           OpsemAux.CurTargetData := ?TD;
+           OpsemAux.CurProducts := _;
+           OpsemAux.Globals := _;
+           OpsemAux.FunTable := _ |}
+           {|
+           Opsem.ECS := {|
+                          Opsem.CurFunction := ?F;
+                          Opsem.CurBB := _;
+                          Opsem.CurCmds := nil;
+                          Opsem.Terminator := _;
+                          Opsem.Locals := _;
+                          Opsem.Allocas := _ |} :: _;
+           Opsem.Mem := _ |} |- _] =>
+  destruct Cfg1 as [S1 TD1 Ps1 gl1 fs1];
+  destruct St1 as [ECs1 M1];
+  destruct TD1 as [los nts];
+  destruct Hsim as [Hwfs [HMinS [Htsym [Heq1 [Htps [HsimECs [Heq2 
+    [Heq3 Heq4]]]]]]]]; subst;
+  destruct ECs1 as [|[F1 B1 cs1 tmn1 lc1 als1] ECs1];
+    try solve [inversion HsimECs];
+  simpl in HsimECs;
+  destruct HsimECs as [HsimEC HsimECs];
+  destruct HsimEC as [HBinF [HFinPs [Htfdef [Heq0 [Heq1 [Hbsim [Heqb1 [Heqb2
+    [Hrsim Htcmds]]]]]]]]]; subst
+end.
+
+Lemma lookup_fdef_sim__block_sim : forall pinfo f1 f2 l0 b2,
+  fdef_simulation pinfo f1 f2 ->
+  lookupBlockViaLabelFromFdef f2 l0 = Some b2 ->
+  exists b1,
+    lookupBlockViaLabelFromFdef f1 l0 = Some b1 /\
+    block_simulation pinfo f1 b1 b2.
+Admitted.
+
+Lemma phinodes_placement_is_correct__sBranch: forall 
+  (pinfo : PhiInfo) (Cfg1 : OpsemAux.Config) (St1 : Opsem.State)
+  (S : system) (TD : TargetData) (Ps : list product) (F : fdef) (B : block)
+  (lc : Opsem.GVsMap) (gl : GVMap) (fs : GVMap) (bid : id) (Cond : value)
+  (l1 : l) (l2 : l) (ECs : list Opsem.ExecutionContext) (Mem : mem) 
+  (als : list mblock) maxb EC1 Cfg1 Cfg2 (Hwfpi: WF_PhiInfo pinfo)
+  (Heq1: Cfg2 = {| OpsemAux.CurSystem := S;
+                   OpsemAux.CurTargetData := TD;
+                   OpsemAux.CurProducts := Ps;
+                   OpsemAux.Globals := gl;
+                   OpsemAux.FunTable := fs |})
+  (Hnoalias: Promotability.wf_State maxb pinfo Cfg1 St1) 
+  (Heq2: EC1 = {| Opsem.CurFunction := F;
+                  Opsem.CurBB := B;
+                  Opsem.CurCmds := nil;
+                  Opsem.Terminator := insn_br bid Cond l1 l2;
+                  Opsem.Locals := lc;
+                  Opsem.Allocas := als |})
+  (Hsim : State_simulation pinfo Cfg1 St1 Cfg2
+            {| Opsem.ECS := EC1 :: ECs;
+               Opsem.Mem := Mem |})
+  (conds : GVsT DGVs) (c : GenericValue) (l' : l) (ps' : phinodes)
+  (cs' : cmds) (tmn' : terminator) (lc' : Opsem.GVsMap)
+  (H : Opsem.getOperandValue TD Cond lc gl = ret conds)
+  (H0 : c @ conds)
+  (H1 : ret block_intro l' ps' cs' tmn' =
+       (if isGVZero TD c
+        then lookupBlockViaLabelFromFdef F l2
+        else lookupBlockViaLabelFromFdef F l1))
+  (H2 : Opsem.switchToNewBasicBlock TD (block_intro l' ps' cs' tmn') B gl lc =
+       ret lc'),
+  exists St1' : Opsem.State,
+     Opsem.sop_star Cfg1 St1 St1' trace_nil /\
+     State_simulation pinfo Cfg1 St1' Cfg2
+     {|Opsem.ECS := {| Opsem.CurFunction := F;
+                       Opsem.CurBB := (block_intro l' ps' cs' tmn');
+                       Opsem.CurCmds := cs';
+                       Opsem.Terminator := tmn';
+                       Opsem.Locals := lc';
+                       Opsem.Allocas := als |} :: ECs;
+       Opsem.Mem := Mem |}.
+Proof.
+  intros. subst.
+  destruct_ctx_br.
+  assert (exists b1,
+    (if isGVZero (los, nts) c
+     then lookupBlockViaLabelFromFdef F1 l2
+     else lookupBlockViaLabelFromFdef F1 l1) = Some b1 /\
+    block_simulation pinfo F1 b1 (block_intro l' ps' cs' tmn')) as Hfind.
+    symmetry in H1.
+    destruct (isGVZero (los, nts) c); 
+      eapply lookup_fdef_sim__block_sim in H1; eauto.
+  destruct Hfind as [b1 [Hfind Htblock]].
+  assert (Htcmds':=Htcmds).
+  apply cmds_simulation_nil_inv in Htcmds'. subst.
+  unfold cmds_simulation in Htcmds.
+  destruct Heqb1 as [l3 [ps3 [cs11 Heqb1]]]; subst.
+  destruct pinfo as
+    [PI_f0 PI_rd0 PI_succs0 PI_preds0 PI_id0 PI_typ0 PI_align0 PI_newids0].
+  simpl in *.
+  remember 
+    (mkPhiInfo PI_f0 PI_rd0 PI_succs0 PI_preds0 PI_id0 PI_typ0 
+                  PI_align0 PI_newids0) as pinfo.
+
+  destruct (fdef_dec PI_f0 F1) as [ e | n]; subst F1.
+  SCase "F is tranformed".
+    assert (PI_newids0 ! l3 <> None) as Hreach.
+      admit. (* reachable *)
+    remember (PI_newids0 ! l3) as R.
+    destruct R as [[[lid pid] sid]|]; try congruence.
+    destruct Htcmds as [_ [_ Htcmds]].
+    assert (exists sc, exists scs, PI_succs0 ! l3 = Some (sc::scs)) 
+      as R2.
+      admit. (* must be of at most one succs *)
+    destruct R2 as [sc [scs Heq]].
+    rewrite Heq in *.
+    assert ([insn_load lid PI_typ0 (value_id PI_id0) PI_align0] <> nil) 
+      as Hwft.
+      intro J. inv J.
+    apply_clear Htcmds in Hwft.
+
+    destruct b1 as [l0 ps0 cs0 tmn0].
+    unfold phinodes_placement_block in Htblock.
+    assert (PI_newids0 ! l0 <> None) as Hreach'.
+      admit. (* reachable *)
+    remember (PI_newids0 ! l0) as R1.
+    destruct R1 as [[[lid' pid'] sid']|]; try congruence.
+    assert (exists prd, exists prds, PI_preds0 ! l0 = Some (prd::prds)) 
+      as R2.
+      admit. (* must be of at most one prds *)
+    destruct R2 as [prd [prds Heq']].
+    rewrite Heq' in *. 
+    inversion Htblock; subst l' ps' cs' tmn'. clear Htblock.
+
+    unfold wf_tmp_value in Hwft. simpl in Hwft.
+    destruct Hwft as [gvsa [gv [Hlkp1 [Hld Hlk2]]]].
+
+    assert (lookupAL _ lc' pid' = Some gv /\
+            lookupAL (GVsT DGVs) lc' PI_id0 = ret gvsa) as Hswitch2.
+      admit. (* switch *)
+    destruct Hswitch2 as [Hlka Hlkb].
+    assert (exists lc1', 
+      Opsem.switchToNewBasicBlock (los, nts) (block_intro l0 ps0 cs0 tmn0)
+        (block_intro l3 ps3 (cs11 ++ nil) (insn_br bid Cond l1 l2)) gl 
+        lc1 = ret lc1' /\
+      reg_simulation pinfo PI_f0 lc1' lc') as Hswitch1.
+      admit. (* switch *)
+    destruct Hswitch1 as [lc1' [Hswitch1 Hrsim']].
+
+    exists (Opsem.mkState 
+             ((Opsem.mkEC PI_f0 (block_intro l0 ps0 cs0 tmn0) cs0 tmn0 lc1' als)
+              ::ECs1) Mem).
+    split.
+    SSCase "opsem".
+      apply OpsemProps.sInsn__implies__sop_star.
+      econstructor; eauto.
+        erewrite simulation__getOperandValue with (lc2:=lc); eauto.
+        apply original_values_arent_tmps with 
+          (instr:=insn_terminator (insn_br bid Cond l1 l2))
+          (B:=block_intro l3 ps3 (cs11 ++ nil) (insn_br bid Cond l1 l2)); 
+          simpl; auto.
+          rewrite Heqpinfo. auto.
+
+          apply andb_true_iff.
+          split; auto.
+            apply terminatorEqB_refl.
+
+    SSCase "sim".
+      assert (blockInFdefB (block_intro l0 ps0 cs0 tmn0) PI_f0)as HBinF'.
+        assert (HuniqF:=HFinPs).
+        eapply wf_system__uniqFdef in HuniqF; eauto.
+        destruct PI_f0 as [[f t i0 a v] bs]. 
+        destruct HuniqF as [HuniqBlocks HuniqArgs].
+        destruct (isGVZero (los,nts) c);
+          apply genLabel2Block_blocks_inv with (f:=fheader_intro f t i0 a v) 
+            in Hfind; auto; destruct Hfind; eauto.
+      repeat (split; eauto 2 using cmds_at_block_tail_next).
+      SSSCase "fsim".
+        rewrite Heqpinfo. simpl.
+        destruct (fdef_dec PI_f0 PI_f0); auto; try congruence.
+
+      SSSCase "bsim".
+        rewrite Heqpinfo. simpl.
+        destruct (fdef_dec PI_f0 PI_f0); try congruence.
+        rewrite <- HeqR1. rewrite Heq'. auto.
+
+      SSSCase "eq".
+        exists l0. exists ps0. exists nil. auto.
+
+      SSSCase "eq".
+        exists l0. 
+        exists (gen_phinode pid' PI_typ0 PI_newids0 (prd :: prds) :: ps0).
+        exists nil. simpl_env. auto.
+
+      SSSCase "csim".
+        rewrite Heqpinfo in *. simpl in *.
+        destruct (fdef_dec PI_f0 PI_f0); try congruence.
+        rewrite <- HeqR1. rewrite Heq'.
+        split; intros.
+          split; auto.
+            intros. 
+            unfold wf_tmp_value. simpl.
+            exists gvsa. exists gv. repeat split; auto.
+        split; intros; congruence.
+        
+  SCase "F isnt tranformed".
+    admit. (* simpl case *)
+Qed.
+
+Ltac destruct_ctx_other :=
+match goal with
+| [Hsim : State_simulation _ ?Cfg1 ?St1
+           {|
+           OpsemAux.CurSystem := _;
+           OpsemAux.CurTargetData := ?TD;
+           OpsemAux.CurProducts := _;
+           OpsemAux.Globals := _;
+           OpsemAux.FunTable := _ |}
+           {|
+           Opsem.ECS := {|
+                          Opsem.CurFunction := ?F;
+                          Opsem.CurBB := _;
+                          Opsem.CurCmds := _::_;
+                          Opsem.Terminator := _;
+                          Opsem.Locals := _;
+                          Opsem.Allocas := _ |} :: _;
+           Opsem.Mem := _ |} |- _] =>
+  destruct Cfg1 as [S1 TD1 Ps1 gl1 fs1];
+  destruct St1 as [ECs1 M1];
+  destruct TD1 as [los nts];
+  destruct Hsim as [Hwfs [HMinS [Htsym [Heq1 [Htps [HsimECs [Heq2 
+    [Heq3 Heq4]]]]]]]]; subst;
+  destruct ECs1 as [|[F1 B1 cs1 tmn1 lc1 als1] ECs1];
+    try solve [inversion HsimECs];
+  simpl in HsimECs;
+  destruct HsimECs as [HsimEC HsimECs];
+  destruct HsimEC as [HBinF [HFinPs [Htfdef [Heq0 [Heq1 [Hbsim [Heqb1 [Heqb2
+    [Hrsim Htcmds]]]]]]]]]; subst
+end.
+
+Lemma SBpass_is_correct__dsLoad: forall (maxb : Values.block) (pinfo : PhiInfo)
+  (Cfg1 : OpsemAux.Config) (St1 : Opsem.State) (Hwfpi : WF_PhiInfo pinfo)
+  (Hnoalias : wf_State maxb pinfo Cfg1 St1) (S : system) (TD : TargetData)
+  (Ps : list product) (F : fdef) (B : block) (lc : Opsem.GVsMap) (gl : GVMap)
+  (fs : GVMap) (id0 : id) (t : typ) (align0 : align) (v : value)
+  (EC : list Opsem.ExecutionContext) (cs : list cmd) (tmn : terminator)
+  (Mem : mem) (als : list mblock) Cfg2
+  (EQ : Cfg2 = {| OpsemAux.CurSystem := S;
+                  OpsemAux.CurTargetData := TD;
+                  OpsemAux.CurProducts := Ps;
+                  OpsemAux.Globals := gl;
+                  OpsemAux.FunTable := fs |})
+  (Hsim : State_simulation pinfo Cfg1 St1 Cfg2
+           {|
+           Opsem.ECS := {|
+                        Opsem.CurFunction := F;
+                        Opsem.CurBB := B;
+                        Opsem.CurCmds := insn_load id0 t v align0 :: cs;
+                        Opsem.Terminator := tmn;
+                        Opsem.Locals := lc;
+                        Opsem.Allocas := als |} :: EC;
+           Opsem.Mem := Mem |})
+  (mps : GVsT DGVs) (mp : GenericValue) (gv : GenericValue)
+  (H : Opsem.getOperandValue TD v lc gl = ret mps)
+  (H0 : mp @ mps) (H1 : mload TD Mem mp t align0 = ret gv),
+  exists St1' : Opsem.State,
+     Opsem.sop_star Cfg1 St1 St1' trace_nil /\
+     State_simulation pinfo Cfg1 St1' Cfg2
+       {|
+       Opsem.ECS := {|
+                    Opsem.CurFunction := F;
+                    Opsem.CurBB := B;
+                    Opsem.CurCmds := cs;
+                    Opsem.Terminator := tmn;
+                    Opsem.Locals := updateAddAL (GVsT DGVs) lc id0
+                                      ($ gv # t $);
+                    Opsem.Allocas := als |} :: EC;
+       Opsem.Mem := Mem |}.
+Proof.
+  intros. subst.
+  destruct_ctx_other.
+
+Admitted.
 
 Lemma phinodes_placement_is_bsim : forall maxb pinfo Cfg1 St1 Cfg2 St2 St2' tr
   (Hwfpi: WF_PhiInfo pinfo) 
@@ -919,64 +1447,85 @@ Proof.
 Case "sReturn".  
 Focus.
   destruct_ctx_return.
-  apply cmds_simulation_nil_ret_inv in Htcmds. subst.
-  apply cmds_simulation_cons_inv in Htcmds'.
-  destruct Htcmds' as [cs2'0 [EQ Htcmds']]; subst.
+  apply cmds_simulation_nil_inv in Htcmds. subst.
+  apply cmds_simulation_non_ldst_cons_inv in Htcmds'; 
+    try solve [
+      destruct Heqb1' as [l3 [ps3 [cs3 Heqb1']]]; subst; eauto |
+      simpl; auto
+    ].
+  destruct Htcmds' as [cs1'0 [EQ Htcmds']]; subst.
+  assert (if fdef_dec (PI_f pinfo) F1
+          then value_has_no_tmps pinfo Result else True) as Hnontmp.
+    apply original_values_arent_tmps with 
+      (instr:=insn_terminator (insn_return rid RetTy Result))(B:=B1); 
+      simpl; try solve [auto | solve_tmnInFdefBlockB].
   eapply returnUpdateLocals_rsim in H1; eauto.
-  destruct H1 as [lc2'' [H1 Hrsim'']].
+  destruct H1 as [lc1'' [H1 Hrsim'']].
   exists 
-    (Opsem.mkState ((Opsem.mkEC F2' B2' cs2'0 tmn2' lc2'' als2')::ECs2) Mem').
+    (Opsem.mkState ((Opsem.mkEC F1' B1' cs1'0 tmn' lc1'' als')::ECs1) Mem').
   split.
     rewrite <- (@trace_app_nil__eq__trace trace_nil).
-    apply OpsemProps.sInsn__implies__sop_plus.
+    apply OpsemProps.sInsn__implies__sop_star.
     constructor; auto.
   
     repeat (split; eauto 2 using cmds_at_block_tail_next).
+      destruct Heqb1' as [l1 [ps1 [cs11 Heqb1']]]; subst.
+      destruct Heqb2' as [l2 [ps2 [cs21 Heqb2']]]; subst.
+      eapply cmds_simulation_stable; eauto.
+      eapply ECs_simulation_tail_stable; eauto.
+Unfocus.
 
 Case "sReturnVoid".
+Focus.
   destruct_ctx_return.
-  eapply cmds_simulation_nil_ret_inv in Htcmds; eauto. subst.
-  apply cmds_simulation_cons_inv in Htcmds'.
-  destruct Htcmds' as [cs2'0 [EQ Htcmds']]; subst.
+  apply cmds_simulation_nil_inv in Htcmds. subst.
+  apply cmds_simulation_non_ldst_cons_inv in Htcmds'; 
+    try solve [
+      destruct Heqb1' as [l3 [ps3 [cs3 Heqb1']]]; subst; eauto |
+      simpl; auto
+    ].
+  destruct Htcmds' as [cs1'0 [EQ Htcmds']]; subst.
   exists 
-    (Opsem.mkState ((Opsem.mkEC F2' B2' cs2'0 tmn2' lc2' als2')::ECs2) Mem').
+    (Opsem.mkState ((Opsem.mkEC F1' B1' cs1'0 tmn' lc1' als')::ECs1) Mem').
   split.
     rewrite <- (@trace_app_nil__eq__trace trace_nil).
-    apply OpsemProps.sInsn__implies__sop_plus.
+    apply OpsemProps.sInsn__implies__sop_star.
     constructor; auto.
   
     repeat (split; eauto 2 using cmds_at_block_tail_next).
+      destruct Heqb1' as [l1 [ps1 [cs11 Heqb1']]]; subst.
+      destruct Heqb2' as [l2 [ps2 [cs21 Heqb2']]]; subst.
+      eapply cmds_simulation_stable; eauto.
+      eapply ECs_simulation_tail_stable; eauto.
+Unfocus.
 
 Case "sBranch". eapply phinodes_placement_is_correct__sBranch; eauto.
 Case "sBranch_uncond". admit.
   (* eapply SBpass_is_correct__dsBranch_uncond; eauto. *)
-Case "sBop". 
+Case "sBop". admit. (* eapply SBpass_is_correct__dsBop; eauto. *)
+Case "sFBop". admit. (* eapply SBpass_is_correct__dsFBop; eauto. *)
+Case "sExtractValue". admit. 
+  (* eapply SBpass_is_correct__dsExtractValue; eauto. *)
+Case "sInsertValue". admit. (* eapply SBpass_is_correct__dsInsertValue; eauto. *)
+Case "sMalloc". admit. (* eapply SBpass_is_correct__dsMalloc; eauto. *)
+Case "sFree". admit. (* eapply SBpass_is_correct__dsFree; eauto. *)
+Case "sAlloca". admit. (* eapply SBpass_is_correct__dsAlloca; eauto. *)
+Case "sLoad". eapply SBpass_is_correct__dsLoad; eauto.
 
 Admitted.
-(*
-eapply SBpass_is_correct__dsBop; eauto.
 
-Case "sFBop". eapply SBpass_is_correct__dsFBop; eauto.
-Case "sExtractValue". eapply SBpass_is_correct__dsExtractValue; eauto.
-Case "sInsertValue". eapply SBpass_is_correct__dsInsertValue; eauto.
-Case "sMalloc". eapply SBpass_is_correct__dsMalloc; eauto.
-Case "sFree". eapply SBpass_is_correct__dsFree; eauto.
-Case "sAlloca". eapply SBpass_is_correct__dsAlloca; eauto.
-Case "sLoad_nptr". eapply SBpass_is_correct__dsLoad_nptr; eauto.
-Case "sLoad_ptr". eapply SBpass_is_correct__dsLoad_ptr; eauto.
-Case "sStore_nptr". eapply SBpass_is_correct__dsStore_nptr; eauto.
-Case "sStore_ptr". eapply SBpass_is_correct__dsStore_ptr; eauto.
+(*
+eapply SBpass_is_correct__dsLoad_nptr; eauto.
+Case "sStore". eapply SBpass_is_correct__dsStore_ptr; eauto.
 Case "sGEP". eapply SBpass_is_correct__dsGEP; eauto.
 Case "sTrunc". eapply SBpass_is_correct__dsTrunc; eauto.
 Case "sExt". eapply SBpass_is_correct__dsExt; eauto.
-Case "sBitcast_nptr". eapply SBpass_is_correct__dsBitcase_nptr; eauto.
-Case "sBitcast_ptr". eapply SBpass_is_correct__dsBitcase_ptr; eauto.
+Case "sBitcast". eapply SBpass_is_correct__dsBitcase_ptr; eauto.
 Case "sInttoptr". eapply SBpass_is_correct__dsInttoptr; eauto.
 Case "sOthercast". eapply SBpass_is_correct__dsOthercast; eauto.
 Case "sIcmp". eapply SBpass_is_correct__dsIcmp; eauto.
 Case "sFcmp". eapply SBpass_is_correct__dsFcmp; eauto.
-Case "sSelect_nptr". eapply SBpass_is_correct__dsSelect_nptr; eauto.
-Case "sSelect_ptr". 
+Case "sSelect". 
   eapply SBpass_is_correct__dsSelect_ptr; eauto.
   unfold prop_reg_metadata.
   destruct (isGVZero TD c); eauto.
